Specify and prove `if_3989404597755436942`
Bringing in changes from https://github.com/EllbellCode/Clear_fork

Co-authored-by: EllbellCode <ellbellcode@gmail.com>

Generated/erc20shim/ERC20Shim/Common/if_3989404597755436942_user.lean
@@ -11,12 +11,171 @@ section
 
 open Clear EVMState Ast Expr Stmt FunctionDefinition State Interpreter ExecLemmas OutOfFuelLemmas Abstraction YulNotation PrimOps ReasoningPrinciple Utilities Generated.erc20shim ERC20Shim
 
-def A_if_3989404597755436942 (s₀ s₉ : State) : Prop := sorry
+def A_if_3989404597755436942 (s₀ s₉ : State) : Prop :=
+  s₉.isOk ∧
+
+  (--Case 1: No initial collision
+    s₀.evm.hash_collision = false →
+  (
+    ( -- Case 1.1 : Reversion
+      preservesEvm s₀ s₉ ∧
+      s₉.evm.reverted = true  ∧
+      s₀["_7"]!! ≠ 0
+    )
+    ∨
+    ( -- Case 1.2 : No Reversion
+      preservesEvm s₀ s₉ ∧
+      s₀["_7"]!! = 0
+    )
+    ∨
+      -- Case 1.3 : Collision in function
+      s₉.evm.hash_collision = true
+  )
+  )
+  ∧
+  (-- Case 2: existing initial collision
+     s₀.evm.hash_collision = true →
+    s₉.evm.hash_collision = true
+  )
 
 lemma if_3989404597755436942_abs_of_concrete {s₀ s₉ : State} :
   Spec if_3989404597755436942_concrete_of_code s₀ s₉ →
   Spec A_if_3989404597755436942 s₀ s₉ := by
-  sorry
+  unfold if_3989404597755436942_concrete_of_code A_if_3989404597755436942
+
+  rcases s₀ with ⟨evm₀, varstore₀⟩ | _ | _ <;> [simp only; aesop_spec; aesop_spec]
+  apply spec_eq
+  rintro hasFuel ⟨s, call_encode, code⟩
+
+  generalize s0_all :
+  (Ok evm₀ varstore₀) = s₀ at *
+
+  unfold A_abi_encode_address_uint256_uint256 at call_encode
+
+  rw [←s0_all] at call_encode
+  rw [insert_of_ok] at call_encode
+  rw [insert_of_ok] at call_encode
+  rw [insert_of_ok] at call_encode
+  simp at call_encode
+  unfold setEvm at call_encode
+  unfold multifill at call_encode
+  simp at call_encode
+  rw [insert_of_ok] at call_encode
+  rw [insert_of_ok] at call_encode
+  unfold lookup! at call_encode
+  unfold State.insert at call_encode
+  simp at call_encode
+
+  generalize general_1 : (Finmap.lookup "_9"
+                                (Finmap.insert "_11" 4
+                                  (Finmap.insert "_10" (Fin.shiftLeft 957625571 226)
+                                    (Finmap.insert "_9" (EVMState.mload evm₀ 64)
+                                      (Finmap.insert "_8" 64
+                                        (Finmap.insert "expr_3"
+                                          (Finmap.lookup "var_value"
+                                              (Finmap.insert "expr_2"
+                                                (Finmap.lookup "_6"
+                                                    (Finmap.insert "expr_1" (Finmap.lookup "var_from" varstore₀).get!
+                                                      varstore₀)).get!
+                                                (Finmap.insert "expr_1" (Finmap.lookup "var_from" varstore₀).get!
+                                                  varstore₀))).get!
+                                          (Finmap.insert "expr_2"
+                                            (Finmap.lookup "_6"
+                                                (Finmap.insert "expr_1" (Finmap.lookup "var_from" varstore₀).get!
+                                                  varstore₀)).get!
+                                            (Finmap.insert "expr_1" (Finmap.lookup "var_from" varstore₀).get!
+                                              varstore₀)))))))).get! = gen_1 at *
+  generalize general_2 : (Finmap.insert "_12" (gen_1 + 4)
+                            (Finmap.insert "_11" 4
+                              (Finmap.insert "_10" (Fin.shiftLeft 957625571 226)
+                                (Finmap.insert "_9" (EVMState.mload evm₀ 64)
+                                  (Finmap.insert "_8" 64
+                                    (Finmap.insert "expr_3"
+                                      (Finmap.lookup "var_value"
+                                          (Finmap.insert "expr_2"
+                                            (Finmap.lookup "_6"
+                                                (Finmap.insert "expr_1" (Finmap.lookup "var_from" varstore₀).get!
+                                                  varstore₀)).get!
+                                            (Finmap.insert "expr_1" (Finmap.lookup "var_from" varstore₀).get!
+                                              varstore₀))).get!
+                                      (Finmap.insert "expr_2"
+                                        (Finmap.lookup "_6"
+                                            (Finmap.insert "expr_1" (Finmap.lookup "var_from" varstore₀).get!
+                                              varstore₀)).get!
+                                        (Finmap.insert "expr_1" (Finmap.lookup "var_from" varstore₀).get!
+                                          varstore₀)))))))) = gen_2 at *
+  generalize general_evm : (mstore evm₀
+            (Finmap.lookup "_9"
+                (Finmap.insert "_10" (Fin.shiftLeft 957625571 226)
+                  (Finmap.insert "_9" (EVMState.mload evm₀ 64)
+                    (Finmap.insert "_8" 64
+                      (Finmap.insert "expr_3"
+                        (Finmap.lookup "var_value"
+                            (Finmap.insert "expr_2"
+                              (Finmap.lookup "_6"
+                                  (Finmap.insert "expr_1" (Finmap.lookup "var_from" varstore₀).get! varstore₀)).get!
+                              (Finmap.insert "expr_1" (Finmap.lookup "var_from" varstore₀).get! varstore₀))).get!
+                        (Finmap.insert "expr_2"
+                          (Finmap.lookup "_6"
+                              (Finmap.insert "expr_1" (Finmap.lookup "var_from" varstore₀).get! varstore₀)).get!
+                          (Finmap.insert "expr_1" (Finmap.lookup "var_from" varstore₀).get! varstore₀))))))).get!
+            (Fin.shiftLeft 957625571 226)) = gen_evm at *
+
+  have s0__ok : (Ok gen_evm gen_2).isOk := by aesop
+  by_cases _3_var : s₀["_7"]!! ≠ 0
+
+  · clr_spec at call_encode
+
+    simp [_3_var] at code
+    obtain ⟨s_ok, ⟨s_preservesEvm, encode, s_no_collision⟩ | s_collision ⟩ := call_encode
+    · obtain ⟨s_evm, ⟨s_varstore, s_all⟩⟩ := State_of_isOk s_ok
+
+      have : Preserved evm₀ gen_evm := by
+        rw[←general_evm]
+        apply mstore_preserved
+
+      have s0_s_preservesEvm : preservesEvm s₀ s := by
+                apply preservesEvm_trans s0__ok
+                aesop
+                aesop
+
+      have s_s9_preservesEvm : preservesEvm s s₉ := by
+        have : Preserved s.evm s₉.evm := by
+          have : (s.evm.account_map    = s₉.evm.account_map ∧
+                          s.evm.hash_collision = s₉.evm.hash_collision ∧
+                          s.evm.execution_env  = s₉.evm.execution_env ∧
+                          s.evm.keccak_map     ≤ s₉.evm.keccak_map) := by
+                          rw[←code]
+                          unfold setEvm
+                          simp [s_all]
+                          rw [insert_of_ok]
+                          unfold evm_revert
+                          unfold evm_return
+                          simp
+
+          simp [Preserved_def]
+          aesop
+        aesop
+
+      unfold setEvm at code
+      simp [s_all] at code
+      split_ands
+      · aesop
+      · intro s0_no_collision
+        left
+        split_ands
+        · apply preservesEvm_trans s_ok
+          all_goals aesop
+        · aesop
+        · aesop
+      · rw[←code]
+        unfold lookup! State.insert evm_revert evm_return
+        simp
+        unfold preservesEvm at s0_s_preservesEvm
+        simp[←s0_all, s_all, Preserved_def] at s0_s_preservesEvm
+        aesop
+    · aesop
+  · aesop
 
 end
 
